test.lean
@@ -1,0 +1,2 @@
+import Mathlib.Data.List.Basic
+example (l : List ℕ) (x : ℕ) : x ∈ l.eraseDups ↔ x ∈ l := by exact List.mem_eraseDups
